

ST-302

Design, Planning and Analysis of Experiments

Dr. (Mrs.) Kirtee Kiran Kamalja
Department of Statistics, School of Mathematical Sciences,
Kavayitri Bahinbai Chaudhari North Maharashtra University,
Jalgaon

Topic 3: Two-way Classification Model with r observations per cell

Testing of hypothesis $H_{01}: \alpha_1^* = \alpha_2^* = \cdots = \alpha_p^*$

- H_{01} can be rewritten in the form of estimable parametric functions.

$$\left. \begin{array}{l} H_{01}: \alpha_1^* = \alpha_2^* \\ \alpha_1^* = \alpha_3^* \\ \vdots \\ \alpha_1^* = \alpha_p^* \end{array} \right\} (p-1) \text{ l.i.e.p.f.}$$

- Let $\alpha_1^* = \alpha_2^* = \cdots = \alpha_p^* = \alpha^*$ (say)
- Here $\alpha_i^* = (\alpha_i + \bar{\gamma}_{i.})$

Testing of hypothesis $H_{01}: \alpha_1^* = \alpha_2^* = \dots = \alpha_p^*$

- **Original model**

Model : $E(y_{ijk}) = \mu + \alpha_i + \beta_j + \gamma_{ij}$

Solution of

Normal equations: $\hat{\mu} = \bar{y}_{...}$,

$$\hat{\alpha}_i = \bar{y}_{i..} - \bar{y}_{...},$$

$$\hat{\beta}_j = \bar{y}_{.j.} - \bar{y}_{...},$$

$$\hat{\gamma}_{ij} = \bar{y}_{ij.} - \bar{y}_{i..} - \bar{y}_{.j.} + \bar{y}_{...}$$

Fitted value : $\hat{y}_{ijk} = \bar{y}_{ij.}$

Testing of hypothesis $H_{01}: \alpha_1^* = \alpha_2^* = \dots = \alpha_p^*$

- **SSE for Original model**

$$SSE = \sum_{i=1}^p \sum_{j=1}^q \sum_{k=1}^r (y_{ijk} - \hat{y}_{ijk})^2$$

$$SSE = \left(\sum_{i=1}^p \sum_{j=1}^q \sum_{k=1}^r y_{ijk}^2 - \frac{y_{...}^2}{pqr} \right) - \left(\sum_{i=1}^p \sum_{j=1}^q \frac{y_{ij.}^2}{r} - \frac{y_{...}^2}{pqr} \right)$$

$$SSE = SST - SS_{cells}$$

$$\text{DF for SSE} : df_{SSE} = pq(r - 1)$$

Testing of hypothesis $H_{01}: \alpha_1^* = \alpha_2^* = \dots = \alpha_p^*$

- **Reduced model**

$$E(y_{ijk}) = \mu + \alpha_i + \beta_j + \gamma_{ij}$$

$$E(y_{ijk}) = \mu + (\alpha_i + \bar{\gamma}_{i.}) + \beta_j + (\gamma_{ij} - \bar{\gamma}_{i.})$$

$$E(y_{ijk}) = \mu + \alpha_i^* + \beta_j + \gamma_{ij}^0 \quad \text{where } \gamma_{ij}^0 = \gamma_{ij} - \bar{\gamma}_{i.}$$

$$E(y_{ijk}) = \mu^0 + \beta_j + \gamma_{ij}^0 \quad \text{where } \mu^0 = \mu + \alpha^*$$

Observe that the parameters γ_{ij}^0 are restricted. That is γ_{ij}^0 are subject to the following p conditions.

$$\begin{aligned} \sum_{j=1}^q \gamma_{ij}^0 &= \sum_{j=1}^q (\gamma_{ij} - \bar{\gamma}_{i.}) \\ &= \gamma_{i.} - q\bar{\gamma}_{i.} = 0, \quad i = 1, 2, \dots, p \end{aligned}$$

Testing of hypothesis $H_{01}: \alpha_1^* = \alpha_2^* = \dots = \alpha_p^*$

- Thus under H_0 model reduces to

$$E(y_{ijk}) = \mu^0 + \beta_j + \gamma_{ij}^0$$

where $\sum_{j=1}^q \gamma_{ij}^0 = 0$, for $i = 1, 2, \dots, p$

- To obtain normal equations and their solutions, minimize the function ϕ with respect to $\hat{\mu}^0, \hat{\beta}_j, \hat{\gamma}_{ij}^0$

$$\phi = \sum_{i=1}^p \sum_{j=1}^q \sum_{k=1}^r (y_{ijk} - \hat{\mu}^0 - \hat{\beta}_j - \hat{\gamma}_{ij}^0)^2$$

subject to the p conditions $\sum_{j=1}^q \gamma_{ij}^0 = 0$, $i = 1, 2, \dots, p$

Testing of hypothesis $H_{01}: \alpha_1^* = \alpha_2^* = \dots = \alpha_p^*$

- To obtain normal equations and their solutions, minimize the function ϕ with respect to $\hat{\mu}^0, \hat{\beta}_j, \hat{\gamma}_{ij}^0$

$$\phi = \sum_{i=1}^p \sum_{j=1}^q \sum_{k=1}^r (y_{ijk} - \hat{\mu}^0 - \hat{\beta}_j - \hat{\gamma}_{ij}^0)^2$$

subject to the p conditions $\sum_{j=1}^q \gamma_{ij}^0 = 0, i = 1, 2, \dots, p$

- The p conditions can be added to the ϕ function to be minimized by adding Langrangian multipliers λ_i for each of the p conditions $\sum_{j=1}^q \gamma_{ij}^0 = 0, i = 1, 2, \dots, p$

Testing of hypothesis $H_{01}: \alpha_1^* = \alpha_2^* = \dots = \alpha_p^* \dots$

- Minimize the function ϕ with respect to $\hat{\mu}^0, \hat{\beta}_j, \hat{\gamma}_{ij}^0, \lambda_i$

$$\phi = \sum_{i=1}^p \sum_{j=1}^q \sum_{k=1}^r (y_{ijk} - \hat{\mu}^0 - \hat{\beta}_j - \hat{\gamma}_{ij}^0)^2 + 2 \sum_{i=1}^p \lambda_i \left(\sum_{j=1}^q \hat{\gamma}_{ij}^0 \right)$$

$$\frac{d\phi}{d\hat{\mu}^0} = 0$$

$$\Rightarrow -2 \sum_{i=1}^p \sum_{j=1}^q \sum_{k=1}^r (y_{ijk} - \hat{\mu}^0 - \hat{\beta}_j - \hat{\gamma}_{ij}^0) = 0$$

$$\Rightarrow y_{...} = pqr\hat{\mu}^0 + pr \sum_{j=1}^q \hat{\beta}_j + r \sum_{i=1}^p \sum_{j=1}^q \hat{\gamma}_{ij}^0 \quad (1)$$

$$\Rightarrow E(y_{...}) = pqr\mu^0 + pr \sum_{j=1}^q \beta_j + r \sum_{i=1}^p \sum_{j=1}^q \gamma_{ij}^0$$

$$\Rightarrow E(\bar{y}_{...}) = \mu + \bar{\alpha} + \bar{\beta} + \bar{\gamma}_{..}$$

Testing of hypothesis $H_{01}: \alpha_1^* = \alpha_2^* = \dots = \alpha_p^*$

$$\phi = \sum_{i=1}^p \sum_{j=1}^q \sum_{k=1}^r (y_{ijk} - \hat{\mu}^0 - \hat{\beta}_j - \hat{\gamma}_{ij}^0)^2 + 2 \sum_{i=1}^p \lambda_i \left(\sum_{j=1}^q \hat{\gamma}_{ij}^0 \right)$$

$$\frac{d\phi}{d\hat{\beta}_j} = 0$$

$$\Rightarrow -2 \sum_{i=1}^p \sum_{k=1}^r (y_{ijk} - \hat{\mu}^0 - \hat{\beta}_j - \hat{\gamma}_{ij}^0), \quad j = 1:q$$

$$\Rightarrow y_{.j.} = pr\hat{\mu}^0 + pr\hat{\beta}_j + r \sum_{i=1}^p \hat{\gamma}_{ij}^0, \quad j = 1:q \quad (\text{A})$$

$$\Rightarrow E(y_{.j.}) = pr\mu^0 + pr\beta_j + r \sum_{i=1}^p \gamma_{ij}, \quad j = 1:q$$

$$\Rightarrow E(\bar{y}_{.j.}) = \mu^0 + \beta_j + \bar{\gamma}_{.j}, \quad j = 1:q$$

Testing of hypothesis $H_{01}: \alpha_1^* = \alpha_2^* = \dots = \alpha_p^*$

$$\phi = \sum_{i=1}^p \sum_{j=1}^q \sum_{k=1}^r (y_{ijk} - \hat{\mu}^0 - \hat{\beta}_j - \hat{\gamma}_{ij}^0)^2 + 2 \sum_{i=1}^p \lambda_i \left(\sum_{j=1}^q \hat{\gamma}_{ij}^0 \right)$$

$$\frac{d\phi}{d\hat{\gamma}_{ij}^0} = 0$$

$$\Rightarrow -2 \sum_{k=1}^r (y_{ijk} - \hat{\mu}^0 - \hat{\beta}_j - \hat{\gamma}_{ij}^0) + 2\lambda_i = 0$$

$$\Rightarrow y_{ij.} = r\hat{\mu}^0 + r\hat{\beta}_j + r\hat{\gamma}_{ij}^0 + \lambda_i, \quad i = 1:p, j = 1:q \quad (\text{B})$$

$$\Rightarrow E(y_{ij.}) = r\mu^0 + r\beta_j + r\gamma_{ij}^0 + \lambda_i, \quad i = 1:p, j = 1:q$$

$$\Rightarrow E(\bar{y}_{ij.}) = \mu^0 + \beta_j + \gamma_{ij}^0 + \lambda_i/r, \quad i = 1:p, j = 1:q$$

Testing of hypothesis $H_{01}: \alpha_1^* = \alpha_2^* = \cdots = \alpha_p^*$

$$\phi = \sum_{i=1}^p \sum_{j=1}^q \sum_{k=1}^r (y_{ijk} - \hat{\mu}^0 - \hat{\beta}_j - \hat{\gamma}_{ij}^0)^2 + 2 \sum_{i=1}^p \lambda_i \left(\sum_{j=1}^q \hat{\gamma}_{ij}^0 \right)$$

$$\frac{d\phi}{d\lambda_i} = 0$$

$$\Rightarrow 2 \sum_{j=1}^q \hat{\gamma}_{ij}^0 = 0$$

$$\Rightarrow \sum_{j=1}^q \hat{\gamma}_{ij}^0 = 0, \quad i = 1:p \quad (C)$$

Testing of hypothesis $H_{01}: \alpha_1^* = \alpha_2^* = \dots = \alpha_p^*$

Normal equations for the reduced model:

$$y_{...} = pqr\hat{\mu}^0 + pr \sum_{j=1}^q \hat{\beta}_j + r \sum_{i=1}^p \sum_{j=1}^q \hat{\gamma}_{ij}^0 \quad (1)$$

$$y_{.j.} = pr\hat{\mu}^0 + pr\hat{\beta}_j + r \sum_{i=1}^p \hat{\gamma}_{ij}^0, \quad j = 1:q \quad (A)$$

$$y_{ij.} = r\hat{\mu}^0 + r\hat{\beta}_j + r\hat{\gamma}_{ij}^0 + \lambda_i, \quad i = 1:p, j = 1:q \quad (B)$$

$$0 = \sum_{j=1}^q \hat{\gamma}_{ij}^0, \quad i = 1:p \quad (C)$$

Number of normal equations $= 1 + p + q + pq$

Number of parameters $= 1 + p + q + pq$

Reduced Model details

- Number of observations= $n = pqr$
- Number of parameters= $1 + p + q + pq$

$$\mu,$$

$$\lambda_1, \lambda_2, \dots, \lambda_p,$$

$$\beta_1, \beta_2, \dots, \beta_q,$$

$$\gamma_{11}^0, \gamma_{12}^0, \dots, \gamma_{1q}^0$$

$$\gamma_{21}^0, \gamma_{22}^0, \dots, \gamma_{2q}^0$$

$$\vdots$$

$$\gamma_{p1}^0, \gamma_{p2}^0, \dots, \gamma_{pq}^0$$

Testing of hypothesis $H_{01}: \alpha_1^* = \alpha_2^* = \dots = \alpha_p^*$

Number of equations which are linearly independent :

- (1) is linearly dependent as $\sum_{i=1}^p (A) = (1)$
- (C) is linearly dependent as $\sum_{i=1}^p (C) = 0$ i.e. $\sum_{i=1}^p \sum_{j=1}^q \hat{\gamma}_{ij}^0 = 0$
- Consider an additional equation $\sum_{j=1}^q \hat{\beta}_j = 0$

$$y_{...} = pqr\hat{\mu}^0 + pr\left(\sum_{j=1}^q \hat{\beta}_j\right) + r\sum_{i=1}^p \left(\sum_{j=1}^q \hat{\gamma}_{ij}^0\right) \quad (1)$$

$$\Rightarrow \hat{\mu} = \bar{y}_{...}$$

Testing of hypothesis $H_{01}: \alpha_1^* = \alpha_2^* = \dots = \alpha_p^*$

$$y_{ij.} = r\hat{\mu}^0 + r\hat{\beta}_j + r\hat{\gamma}_{ij}^0 + \lambda_i, \quad i = 1:p, j = 1:q \quad (\text{B})$$

- Summing equations in (B) over j and then using (C)

$\sum_{j=1}^q (A)$ along with (C)

$$\Rightarrow y_{i..} = qr\hat{\mu}^0 + r \sum_{j=1}^q \hat{\beta}_j + r \sum_{j=1}^q \hat{\gamma}_{ij}^0 + q\lambda_i$$

$$\Rightarrow q\lambda_i = y_{i..} - qr\hat{\mu}^0$$

$$\Rightarrow \frac{\lambda_i}{r} = \bar{y}_{i..} - \hat{\mu}^0 \quad \Rightarrow \quad \lambda_i = r(\bar{y}_{i..} - \bar{y}_{...})$$

Testing of hypothesis $H_{01}: \alpha_1^* = \alpha_2^* = \dots = \alpha_p^*$

$$\lambda_i = r(\bar{y}_{i..} - \bar{y}_{...}), \quad i = 1:p$$

Substituting in (B)

$$y_{ij.} = r\hat{\mu}^0 + r\hat{\beta}_j + r\hat{\gamma}_{ij}^0 + \lambda_i \quad (\text{B})$$

$$\Rightarrow y_{ij.} = r\hat{\mu}^0 + r\hat{\beta}_j + r\hat{\gamma}_{ij}^0 + r(\bar{y}_{i..} - \bar{y}_{...}) \quad i = 1:p, j = 1:q$$

$$\Rightarrow r\hat{\gamma}_{ij}^0 = y_{ij.} - r\hat{\mu}^0 - r\hat{\beta}_j - r(\bar{y}_{i..} - \bar{y}_{...})$$

$$\Rightarrow \hat{\gamma}_{ij}^0 = \bar{y}_{ij.} - \hat{\mu}^0 - \hat{\beta}_j - (\bar{y}_{i..} - \bar{y}_{...})$$

Testing of hypothesis $H_{01}: \alpha_1^* = \alpha_2^* = \dots = \alpha_p^*$

$$\Rightarrow \hat{\gamma}_{ij}^0 = (\bar{y}_{ij.} - \bar{y}_{...}) - (\bar{y}_{.j.} - \bar{y}_{...}) - (\bar{y}_{i..} - \bar{y}_{...})$$

$$\Rightarrow \hat{\gamma}_{ij}^0 = \bar{y}_{ij.} - \bar{y}_{i..} - \bar{y}_{.j.} + \bar{y}_{...}$$

Solution of normal equations for the reduced model:

$$E(y_{ijk}) = \mu^0 + \beta_j + \gamma_{ij}^0 \text{ subject to } \sum_{j=1}^q \gamma_{ij}^0 = 0, \quad i = 1, 2, \dots, p$$

- $\hat{\mu}^0 = \bar{y}_{...}$,
- $\hat{\beta}_j = \bar{y}_{.j.} - \bar{y}_{...}$
- $\hat{\gamma}_{ij}^0 = \bar{y}_{ij.} - \bar{y}_{i..} - \bar{y}_{.j.} + \bar{y}_{...}$

Testing of hypothesis $H_{01}: \alpha_1^* = \alpha_2^* = \dots = \alpha_p^*$

Fitted value of the reduced model:

$$\begin{aligned}\hat{y}_{ijk} &= \hat{\mu}^0 + \hat{\beta}_j + \hat{\gamma}_{ij}^0 \\ &= \bar{y}_{...} + (\bar{y}_{.j.} - \bar{y}_{...}) + (\bar{y}_{ij.} - \bar{y}_{i..} - \bar{y}_{.j.} + \bar{y}_{...}) \\ &= \bar{y}_{...} + (\bar{y}_{ij.} - \bar{y}_{...}) - (\bar{y}_{i..} - \bar{y}_{...})\end{aligned}$$

Testing of hypothesis $H_{01}: \alpha_1^* = \alpha_2^* = \dots = \alpha_p^* \dots$

$$= SSE_c$$

$$= \sum_{i=1}^p \sum_{j=1}^q \sum_{k=1}^r (y_{ijk} - \hat{y}_{ijk})^2$$

$$= \sum_{i=1}^p \sum_{j=1}^q \sum_{k=1}^r \left(y_{ijk} - \left(\bar{y}_{...} + (\bar{y}_{ij.} - \bar{y}_{...}) - (\bar{y}_{i..} - \bar{y}_{...}) \right) \right)^2$$

$$= \sum_{i=1}^p \sum_{j=1}^q \sum_{k=1}^r \left((y_{ijk} - \bar{y}_{...}) - (\bar{y}_{ij.} - \bar{y}_{...}) + (\bar{y}_{i..} - \bar{y}_{...}) \right)^2$$

$$= \sum_{i=1}^p \sum_{j=1}^q \sum_{k=1}^r (y_{ijk} - \bar{y}_{...})^2 - \sum_{i=1}^p \sum_{j=1}^q \sum_{k=1}^r (\bar{y}_{ij.} - \bar{y}_{...})^2 \\ + \sum_{i=1}^p \sum_{j=1}^q \sum_{k=1}^r (\bar{y}_{i..} - \bar{y}_{...})^2$$

$$= SST - SS_{cells} + SSA$$

Testing of hypothesis $H_{01}: \alpha_1^* = \alpha_2^* = \dots = \alpha_p^* \dots$

- **SSH_0 for the hypothesis**

$$SSH_0$$

$$= SSE_c - SSE$$

$$= (SST - SS_{cells} + SSA) - (SST - SS_{cells})$$

$$= SSA$$

$$= \sum_{i=1}^p \sum_{j=1}^q \sum_{k=1}^r (\bar{y}_{i..} - \bar{y}_{...})^2$$

$$= \frac{\sum_{i=1}^p y_{i..}^2}{qr} - \frac{y_{...}^2}{pqr}$$

Testing of hypothesis $H_{01}: \alpha_1^* = \alpha_2^* = \dots = \alpha_p^* \dots$

- **Test Statistic**

$$SSH_0 = \sum_{i=1}^p qr(\bar{y}_{i..} - \bar{y}_{...})^2 \sim \sigma^2 \chi_{(p-1)}^2$$

$$SSE = \sum_{i=1}^p \sum_{j=1}^q \sum_{k=1}^r (y_{ijk} - \bar{y}_{ij.})^2$$

$$SSE \sim \sigma^2 \chi_{pq(r-1)}^2$$

$$MSH_0 = \sum_{i=1}^p qr(\bar{y}_{i..} - \bar{y}_{...})^2 / (p - 1)$$

$$MSE = SSE / (pq(r - 1))$$

$$\text{Test - Statistic} = \frac{MSH_0}{MSE} \sim F_{(p-1), pq(r-1)}$$

Testing of hypothesis $H_{02}: \beta_1^* = \beta_2^* = \cdots = \beta_q^*$

- **Test Statistic**

$$SSH_0 = \sum_{j=1}^q pr(\bar{y}_{.j.} - \bar{y}_{...})^2 \sim \sigma^2 \chi_{(q-1)}^2$$

$$SSE = \sum_{i=1}^p \sum_{j=1}^q \sum_{k=1}^r (y_{ijk} - \bar{y}_{ij.})^2$$

$$SSE \sim \sigma^2 \chi_{pq(r-1)}^2$$

$$MSH_0 = \sum_{j=1}^q pr(\bar{y}_{.j.} - \bar{y}_{...})^2 / (q - 1)$$

$$MSE = SSE / (pq(r - 1))$$

$$Test - Statistic = \frac{MSH_0}{MSE} \sim F_{(q-1), pq(r-1)}$$

Estimation of error variance

$$SSE = \sum_{i=1}^p \sum_{j=1}^q \sum_{k=1}^r (y_{ijk} - \bar{y}_{ij.})^2$$

$$SSE \sim \sigma^2 \chi_{(pq(r-1))}^2$$

$$E(SSE) = \sigma^2 (pq(r-1))$$

$$E\left(\frac{SSE}{pq(r-1)}\right) = \sigma^2$$

$$E(MSE) = \sigma^2 \quad \because \text{MSE} = SSE / pq(r-1)$$

$$\hat{\sigma}^2 = MSE = \frac{\sum_{i=1}^p \sum_{j=1}^q \sum_{k=1}^r (y_{ijk} - \bar{y}_{ij.})^2}{pq(r-1)}$$

Thus $\hat{\sigma}^2$ is an unbiased estimator of σ^2 (i.e. Error variance)

ANOVA

Source of vari.	Degrees of Freedom	Sum of squares	Mean SS	F-ratio	Hypothesis
F-A	$(p - 1)$	$SS_A = \frac{\sum_{i=1}^p y_{i..}^2}{qr} - \frac{y_{...}^2}{pqr}$	$MSA = \frac{SSA}{p - 1}$	$\frac{MS_A}{MSE}$	$H_{01}: \alpha_1^* = \dots = \alpha_p^*$
F-B	$(q - 1)$	$SS_B = \frac{\sum_{j=1}^q y_{.j.}^2}{pr} - \frac{y_{...}^2}{pqr}$	$MSB = \frac{SSB}{q - 1}$	$\frac{MS_B}{MSE}$	$H_{02}: \beta_1^* = \dots = \beta_q^*$
Int-AB	$(p - 1) \times (q - 1)$	$SS_{AB} = SS_{cells} - SS_A - SS_B$	$MS_{AB} = \frac{SS_{AB}}{(p - 1)(q - 1)}$	$\frac{MS_{AB}}{MSE}$	$H_{03}: \gamma_{ij}^* = 0 \quad \forall i, j$
Error	$pq(r - 1)$	$SSE = SST - SS_{cells}$	$MSE = \frac{SSE}{pq(r - 1)}$		
Total	$(pqr - 1)$	$SST = \sum_{i,j,k} y_{ijk}^2 - \frac{y_{...}^2}{pqr}$			

ANOVA

- $SS_{cells} = \frac{\sum_{i,j} y_{ij}^2}{r} - \frac{y_{...}^2}{pqr}$
- $\frac{MSA}{MSE} \sim F_{(p-1), pq(r-1)}$
- $\frac{MSB}{MSE} \sim F_{(q-1), pq(r-1)}$
- $\frac{MSAB}{MSE} \sim F_{(q-1)(q-1), pq(r-1)}$
- Further $E(MSE) = \sigma^2$, that is MSE is unbiased estimator of σ^2

Decision about TOH

- p-value for $H_{01} = 1 - P \left(F_{(p-1),pq(r-1)} \leq \frac{MS_A}{MSE} \right)$
- p-value for $H_{02} = 1 - P \left(F_{(q-1),pq(r-1)} \leq \frac{MS_B}{MSE} \right)$
- p-value for $H_{03} = 1 - P \left(F_{(p-1)(q-1),pq(r-1)} \leq \frac{MS_{AB}}{MSE} \right)$
- If p-value for $H_{01} < \alpha$ then reject H_{01}
- If p-value for $H_{02} < \alpha$ then reject H_{02}
- If p-value for $H_{03} < \alpha$ then reject H_{03}

Testing the hypothesis with individual epf.

- $H_0: \alpha_1^* = \alpha_2^*$
- Rewrite H_0 as $\alpha_1^* - \alpha_2^* = 0$
- $\widehat{\alpha_1^* - \alpha_2^*} = \bar{y}_{1..} - \bar{y}_{2..} \sim N(\alpha_1^* - \alpha_2^*, \text{var}(\widehat{\alpha_1^* - \alpha_2^*}))$
- $\bar{y}_{1..} - \bar{y}_{2..} \sim N\left(\alpha_1^* - \alpha_2^*, \frac{2\sigma^2}{qr}\right)$
- $\frac{(\bar{y}_{1..} - \bar{y}_{2..}) - (\alpha_1^* - \alpha_2^*)}{\sqrt{\frac{2\sigma^2}{qr}}} \sim N(0, 1)$
- $\left\{ \frac{(\bar{y}_{1..} - \bar{y}_{2..}) - (\alpha_1^* - \alpha_2^*)}{\sqrt{\frac{2\sigma^2}{qr}}} \right\}^2 \sim \chi^2_{(1)}$

Testing the hypothesis with individual epf.

- Under the null hypothesis $\alpha_1^* - \alpha_2^* = 0$.
- Hence $SSH_0 = \frac{(\bar{y}_{1..} - \bar{y}_{2..})^2}{\left(\frac{2}{qr}\right)} \sim \sigma^2 \chi_{(1)}^2$
- $SSE = \sum_{i,j,k} (y_{ijk} - \bar{y}_{ij.})^2 \sim \sigma^2 \chi_{(pq(r-1))}^2$
- Further SSH_0 is independently distributed of SSE.
- Hence test statistic is:

$$\frac{\frac{(\bar{y}_{1..} - \bar{y}_{2..})^2}{\left(\frac{2}{qr}\right)}}{MSE} \sim F_{1, (pq(r-1))}$$

Testing the hypothesis with individual epf.

- There is no interaction between first level of factor A and second level of factor B
- $H_0: \gamma_{12}^* = 0$
- $\hat{\gamma}_{12}^* = \bar{y}_{12..} - \bar{y}_{1..} - \bar{y}_{2..} + \bar{y}_{...} \sim N(\gamma_{12}^*, \text{var}(\hat{\gamma}_{12}^*))$

$$(\bar{y}_{12..} - \bar{y}_{1..} - \bar{y}_{2..} + \bar{y}_{...}) \sim N\left(\gamma_{12}^*, \frac{\sigma^2(p-1)(q-1)}{pqr}\right)$$

$$\bullet \left\{ \frac{(\bar{y}_{12..} - \bar{y}_{1..} - \bar{y}_{2..} + \bar{y}_{...}) - \gamma_{12}^*}{\sqrt{\frac{\sigma^2(p-1)(q-1)}{pqr}}} \right\}^2 \sim \chi_{(1)}^2$$

Testing the hypothesis with individual epf.

- Under the null hypothesis $\frac{(\bar{y}_{12..} - \bar{y}_{1..} - \bar{y}_{2..} + \bar{y}_{...})^2}{\frac{(p-1)(q-1)}{pqr}} \sim \sigma^2 \chi^2_{(1)}$
- $SSE = \sum_{i,j,k} (y_{ijk} - \bar{y}_{ij.})^2 \sim \sigma^2 \chi^2_{(pq(r-1))}$
- Further SSH_0 is independently distributed of SSE.
- Hence test statistic is:

$$\frac{\frac{(\bar{y}_{12..} - \bar{y}_{1..} - \bar{y}_{2..} + \bar{y}_{...})^2}{\frac{(p-1)(q-1)}{pqr}}}{MSE} \sim F_{1, (pq(r-1))}$$

General test statistic for Testing the individual epf.

- $H_0: \underline{\lambda}' \underline{\beta} = d$

- As $\underline{\lambda}' \hat{\underline{\beta}} \sim N \left(\underline{\lambda}' \underline{\beta}, \text{var} \left(\underline{\lambda}' \hat{\underline{\beta}} \right) \right) \Rightarrow SSH_0 = \frac{(\underline{\lambda}' \hat{\underline{\beta}} - d)^2}{\text{var}(\underline{\lambda}' \hat{\underline{\beta}})} \sim \chi^2_{(1)}$

- $\frac{SSE}{\sigma^2} \sim \chi^2_{pq(r-1)}$

- SSH_0 is independently distributed of SSE

- Hence *test – statistic* $\sim F_{1,pq(r-1)}$ distribution and is:

$$\frac{\left(BLUE(\underline{\lambda}' \underline{\beta}) - \text{hypothetical value of } \underline{\lambda}' \underline{\beta} \right)^2 / \left(\text{var}(\underline{\lambda}' \hat{\underline{\beta}}) \text{ without } \sigma^2 \right)}{MSE}$$

What we have studied

- GLM for two-way classification model with interaction and r observations per cell
- Normal equations and their solutions
- Estimability conditions for linear parametric functions
- Estimable parametric functions, their BLUEs and variances of BLUEs.
- Rank of error space and estimation space
- A set of linearly independent estimable parametric functions
- Fitted value of y_{ij} , SSE and an unbiased estimator of error variance
- Testing of hypothesis: No interaction effect, equality of all row/column effects
- Testing of hypothesis: single epf
- ANOVA table specifying the hypothesis to be tested against each row of it.